proof/crypto_stream/chacha20/ref/ChaCha20_sref_proof.ec
@@ -1,4 +1,4 @@
-require import List Jasmin_model Int IntDiv IntExtra CoreMap.
+require import AllCore List Jasmin_model Int IntDiv IntExtra CoreMap.
 import IterOp.
 require import ChaCha20_Spec ChaCha20_pref ChaCha20_pref_proof ChaCha20_sref.
 require import Array3 Array8 Array16.
@@ -91,16 +91,251 @@ equiv sum_states : ChaCha20_pref.M.sum_states ~ ChaCha20_sref.M.sum_states :
   res{1} = res{2}.`1.[15 <- res{2}.`2].
 proof.
   proc => /=.  
-  admit.
+  unroll for{1} 2; unroll for{2} 2.
+  conseq (_: all_eq k{1} k{2}.[15 <- k15{2}]).
+  + by move=> &1 &2 _ k1 k2 k15 /Array16.all_eq_eq. 
+  wp; skip => />.
+qed.
+
+require import Real.
+
+
+theory Loop.
+
+type t.
+op c : int.
+
+module type AdvLoop = {
+  proc body(t:t, i:int) : t
+}.
+
+
+module Loop(B:AdvLoop) = {
+  proc loop1 (t:t, n:int) = {
+    var i;
+    i = 0;
+    while (i < n) {
+      t <@ B.body(t,i);
+      i <- i + 1;
+    }
+    return t;
+  }
+
+  proc loopk (t:t, n:int, k:int) = {
+    var i, j;
+    i = 0;
+    while (i < n) {
+      j = 0;
+      while (j < k) {
+        t <@ B.body(t, k * i + j);
+        j <- j + 1;
+      }
+      i <- i + 1;
+    }
+    return t;
+  }
+
+  proc loopc (t:t, n:int) = {
+    var i, j;
+    i = 0;
+    while (i < n) {
+      j = 0;
+      while (j < c) {
+        t <@ B.body(t, c * i + j);
+        j <- j + 1;
+      }
+      i <- i + 1;
+    }
+    return t;
+  }
+
+}.
+
+section.
+declare module B:AdvLoop.
+
+axiom B_ll : islossless B.body.
+
+equiv loop1_loopk : Loop(B).loop1 ~ Loop(B).loopk : ={t, glob B} /\ n{1} = (k * n){2} /\ 0 < k{2}==> ={res, glob B}.
+proof.
+  proc.
+  async while [ (fun r => i%r < r), (i{1}+k{2})%r ] 
+              [ (fun r => i%r < r), (i{2} + 1)%r ]
+  
+              ( (i < n){1} /\ (i < n){2}) 
+              (!(i < n){2}) : 
+              (={t, glob B} /\ (0 <= i <= n){2} /\ 0 < k{2} /\ n{1} = (k * n){2} /\ i{1} = k{2} * i{2}).
+  + smt(). + smt (). + smt().
+  + move=> &m2;exfalso;smt().
+  + move=> &m1;exfalso;smt().
+  + move=> v1 v2.
+    rcondt{2} 1; 1: by auto => /> /#.
+    rcondf{2} 4; 1: by auto; conseq (_: true);auto.
+    exlim i{2} => i2.
+    wp;while (={t,glob B} /\ i{1} = k{2}*i{2} + j{2} /\ 0 <= i{2} < n{2} /\ 
+              0 <= j{2} <= k{2} /\ v1 = (k{2} * i2 + k{2})%r /\ i{2} = i2 /\ n{1} = (k * n){2}).
+    + wp;call (_: true);skip => /> &2 h0i hin h0j hjk.
+      rewrite !RealExtra.lt_fromint => h1 h2 h3.
+      have := StdOrder.IntOrder.ler_wpmul2l k{2} _ i{2} (n{2} - 1); smt(). 
+    by wp;skip => /> /#.
+  + by while (true) (n - i);auto;1:call B_ll;auto => /> /#.
+  + while (true) (n-i);2: by auto=>/#.
+    by move=> z;wp; while (true) (k - j);auto;1:call B_ll;auto => /> /#.
+  by auto.
+qed.
+
+equiv loopk_loopc : Loop(B).loopk ~ Loop(B).loopc : ={n,t, glob B} /\ k{1} = c ==> ={res, glob B}.
+proof.
+  proc => /=.
+  while (={glob B, i, t, n} /\ k{1} = c);2: by auto.
+  wp;while (={glob B, i, j, t, n} /\ k{1} = c);2: by auto.
+  by wp;call (_:true);skip.
+qed.
+
+lemma loop1_loopc : 0 < c =>
+  equiv [Loop(B).loop1 ~ Loop(B).loopc : ={t, glob B} /\ n{1} = (c * n){2} ==> ={res, glob B}].
+proof.
+  move=> hc.
+  transitivity Loop(B).loopk
+    (={t, glob B} /\ n{1} = c * n{2} /\ k{2} = c ==> ={res, glob B})
+    (={n,t, glob B} /\ k{1} = c ==> ={res, glob B}).
+  + by move=> /> &1 &2 *; exists (glob B){2} (t{1},n{2}, c).
+  + by move=> />.
+  + by conseq loop1_loopk => /> /#. 
+  by conseq loopk_loopc.  
+qed.
+
+end section.
+
+end Loop.
+
+clone import Loop as Loop0 with
+   type t <- W64.t * W64.t * W32.t Array16.t,
+   op c <- 4.
+
+op inv_ptr (output plain:W64.t) (len:W32.t) = 
+  (to_uint plain + to_uint len < to_uint output || to_uint output <= to_uint plain) /\
+   to_uint output + to_uint len < W64.modulus /\
+   to_uint plain + to_uint len < W64.modulus.
+
+lemma inv_ptr_disj len output plain i1 i2:
+  inv_ptr output plain len =>
+  0 <= i1 <= to_uint len =>
+  0 <= i2 <= to_uint len =>
+  i1 < i2 => 
+  plain + W64.of_int i2 <> output + W64.of_int i1.
+proof.
+  rewrite /inv_ptr /= => [#] h1 h2 h3 hi1 hi2 hlti.
+  rewrite eq_sym -W64.WRingA.eqr_sub W64.WRingA.subr_eq -W64.WRingA.addrA
+     (W64.WRingA.addrC _ (W64.of_int i2)) /=; apply /negP => ->>.
+  have hii: to_uint (W64.of_int (i2 - i1)) = i2 - i1.
+  + by rewrite W64.to_uint_small //=;have /= /#:= W32.to_uint_cmp len.
+  have /# :  to_uint (plain + (W64.of_int (i2 - i1))) = to_uint plain + (i2 - i1).
+  by rewrite W64.to_uintD_small hii /#.
+qed.
+
+module Body = {
+  proc body (t: W64.t * W64.t * W32.t Array16.t, i:int) = {
+    var output, plain, k;
+    (output, plain, k) <- t;
+    Glob.mem <-                
+       storeW8 Glob.mem (output + (of_int i)%W64)       
+          (get8 ((init32 (fun (i0 : int) => k.[i0])))%WArray64 i `^` loadW8 Glob.mem (plain + (of_int i)%W64));
+    return t;
+  }
+}.
+
+lemma load_storeW8 m p1 p2 w: 
+  loadW8 (storeW8 m p1 w) p2 = if p2 = p1 then w else loadW8 m p2.
+proof. by rewrite /loadW8 storeW8E Jasmin_memory.get_setE. qed.
+
+equiv store_store32 len0 : ChaCha20_pref.M.store ~ ChaCha20_pref.M.store32 : 
+  ={Glob.mem, k, output, plain, len} /\ W32.of_int 64 \ule len{1} /\
+  (inv_ptr output plain len){1} /\ len{1} = len0
+  ==>
+  ={Glob.mem, res} /\ (inv_ptr res.`1 res.`2 res.`3){1} /\ res{1}.`3 = len0 - W32.of_int 64.
+proof.
+  proc.
+  inline ChaCha20_pref.M.update_ptr;wp => /=.
+  transitivity{1} { Loop(Body).loop1((output, plain, k), 64);}
+       (={Glob.mem, output, plain, len, k} /\ (of_int 64)%W32 \ule len{1} ==> ={Glob.mem, output, plain, len, k} /\ i{1} = 64)
+       (={Glob.mem, k, output, plain, len} /\
+         ((of_int 64)%W32 \ule len{1}) /\ inv_ptr output{1} plain{1} len{1} /\ len{1} = len0 ==>
+        ={Glob.mem, output, plain, len} /\ inv_ptr (output{1} + (of_int 64)%W64) (plain{1} + (of_int 64)%W64) (len{1} - (of_int 64)%W32) /\
+        len{1} = len0).
+  + by move=> /> &2 *;exists Glob.mem{2} k{2} len{2} output{2} plain{2}. 
+  + by move=> />.
+  + inline *.
+    while ( ={Glob.mem, output, plain, len, k} /\ i{1} = i0{2} /\ 0 <= i{1} <= 64 /\ (t = (output, plain, k)){2} /\ 64 <= to_uint len{1} /\ n0{2} = 64).
+    + by auto => /> &2 h1 h2 h3;rewrite !W32.ultE !W32.to_uint_small /= /#.
+    by auto => /> &2;rewrite W32.uleE W32.ultE /= /#.
+  transitivity{1} { Loop(Body).loopc((output, plain, k), 16);}
+       (={Glob.mem, output, plain, len, k} ==> ={Glob.mem, output, plain, len, k})
+       (={Glob.mem, k, output, plain, len} /\
+         ((of_int 64)%W32 \ule len{1}) /\ inv_ptr output{1} plain{1} len{1} /\ len{1} = len0 ==>
+        ={Glob.mem, output, plain, len} /\ inv_ptr (output{1} + (of_int 64)%W64) (plain{1} + (of_int 64)%W64) (len{1} - (of_int 64)%W32) /\
+        len{1} = len0).
+  + by move=> /> &2 *;exists Glob.mem{2} k{2} len{2} output{2} plain{2}. 
+  + by move=> />.
+  + by call (loop1_loopc Body _ _);[islossless | | skip].
+  inline *;wp.
+  while ( ={Glob.mem, k, output, plain, len} /\ inv_ptr output{1} plain{1} len{1} /\ 64 <= to_uint len{1} /\
+          n0{1} = 16 /\ i0{1} = i{2} /\  0 <= i{2} /\ (t = (output, plain, k)){1}).
+  + unroll for {1} 2;wp;skip => |> &2 h1 h2 h3 h4. 
+    pose ini := WArray64.init32 (fun (i0 : int) => k{2}.[i0]).
+    split; 2: smt().
+    have b0 : 0 <= 4 * i{2} <= to_uint len{2} by smt().
+    have b1 : 0 <= 4 * i{2} + 1 <= to_uint len{2} by smt().
+    have b2 : 0 <= 4 * i{2} + 2 <= to_uint len{2} by smt().
+    have b3 : 0 <= 4 * i{2} + 3 <= to_uint len{2} by smt().
+    do 6!rewrite load_storeW8 (inv_ptr_disj len{2}) // 1:-StdOrder.IntOrder.ltr_subl_addl 1:/# /=. 
+    rewrite -load4u8.
+    have -> : k{2}.[i{2}] = pack4 [get8 ini (4 * i{2}); get8 ini (4 * i{2} + 1);
+                                get8 ini (4 * i{2} + 2); get8 ini (4 * i{2} + 3)].
+    + have <- := W4u8.unpack8K k{2}.[i{2}].
+      congr; apply W4u8.Pack.all_eq_eq.
+      rewrite /all_eq /get8 /ini /init32 /= !WArray64.initiE 1..4:/# /=.
+      by rewrite mulzC !modzMDl /= modzMl mulzK 1:// !divzMDl. 
+    by rewrite /= store4u8.    
+  wp;skip => /> &2 ^ h0;rewrite W32.uleE /= => /> h1 h2 h3 h4 i ??. 
+  rewrite W32.to_uintB 1:// /=.
+  by rewrite W64.to_uintD_small 1:/# W64.to_uintD_small 1:/# /= /#. 
 qed.
 
 equiv store len0 : ChaCha20_pref.M.store ~ ChaCha20_sref.M.store :
   ={Glob.mem} /\ output{1} = s_output{2} /\ plain{1} = s_plain{2} /\ len{1} = s_len{2} /\
-  len{1} = len0 /\ k{1} = k{2}.[15 <- k15{2}] 
+  W32.of_int 64 \ule len{1} /\ (inv_ptr output plain len){1} /\ len{1} = len0 /\
+  k{1} = k{2}.[15 <- k15{2}] 
   ==>
-  ={Glob.mem, res} /\ res{2}.`3 = len0 - W32.of_int 64.
+  ={Glob.mem, res} /\ (inv_ptr res.`1 res.`2 res.`3){1} /\ res{2}.`3 = len0 - W32.of_int 64.
 proof.
-  admit.
+  transitivity ChaCha20_pref.M.store32
+    (={Glob.mem, k, output, plain, len} /\ W32.of_int 64 \ule len{1} /\
+     (inv_ptr output plain len){1} /\ len{1} = len0
+     ==>
+     ={Glob.mem, res} /\ (inv_ptr res.`1 res.`2 res.`3){1} /\ res{1}.`3 = len0 - W32.of_int 64)
+    (={Glob.mem} /\ output{1} = s_output{2} /\ plain{1} = s_plain{2} /\ len{1} = s_len{2} /\ k{1} = k{2}.[15 <- k15{2}]
+     ==> 
+     ={Glob.mem, res}).
+  + move=> /> *; by exists Glob.mem{2} (s_output, s_plain, s_len, k.[15 <- k15]){2}.
+  + by move=> />.
+  + by apply (store_store32 len0).
+  proc => /=.  
+  sim.
+  seq 0 3 : (#pre /\ (s_k.[0] = k.[12] /\ s_k.[1] = k.[13] /\ s_k.[2] = k.[14]){2}).
+  + by unroll for{2} 3; wp;skip => />.
+  sp 0 3.
+  splitwhile {1} 2 : (i < 12).
+  seq 2 2: (={Glob.mem, output, plain, len} /\ k{1}.[12] = s_k{2}.[0] /\ 
+             k{1}.[13] = s_k{2}.[1] /\ k{1}.[14] = s_k{2}.[2] /\ k{1}.[15] = k15{2} /\ i{1} = 12).
+  + by while (={i} /\ #{/~i{1}}post /\ (0 <= i{1} <= 12) /\ (forall j, i{1} <= j < 12 => k{1}.[j] = k{2}.[j]));
+     wp;skip; smt(Array16.get_setE).
+  rcondt{1} 1; 1:by auto. 
+  rcondt{1} 3; 1:by auto. 
+  rcondt{1} 5; 1:by auto. 
+  rcondt{1} 7; 1:by auto. 
+  rcondf{1} 9; 1:by auto. 
+  by unroll for{2} 5; unroll for{2} 2; wp;skip => /> &1 &2 -> -> ->.
 qed.
 
 equiv store_last : ChaCha20_pref.M.store ~ ChaCha20_sref.M.store_last :
@@ -109,7 +344,22 @@ equiv store_last : ChaCha20_pref.M.store ~ ChaCha20_sref.M.store_last :
   ==>
   ={Glob.mem} /\ res{1}.`3 = W32.of_int 0.
 proof.
-  admit.
+  proc => /=.
+  inline *;wp.
+  seq 0 8 :  (={Glob.mem, output, plain, len} /\ W32.to_uint len{1} < 64 /\ k{1} = s_k{2}).
+  + conseq (_ : ={Glob.mem, output, plain, len} /\ W32.to_uint len{1} < 64 /\ Array16.all_eq k{1} s_k{2} ).
+    + by move=> |> &2 ???; apply Array16.all_eq_eq.
+    by unroll for{2} 3;wp;skip => /> &2;rewrite W32.ultE.
+  while (#pre /\ j{2} = W64.of_int i{1} /\ 0 <= i{1} <= W32.to_uint len{1}).
+  + wp;skip => /> &1 &2 ???; rewrite !W32.ultE W32.to_uint_small /= 1:/#.
+    rewrite W8.xorwC /=.
+    rewrite W64.to_uint_small //= 1:/# !W2u32.to_uint_truncateu32.
+    rewrite !W64.to_uint_small //= 1,2:/#.
+    by rewrite W32.to_uint_small //= 1:/#; smt(modz_small).
+  wp;skip => /> &2 ?.
+  case: (W32.to_uint_cmp len{2}) => /> ?? i; rewrite W32.ultE => + *. 
+  rewrite W32.to_uint_small /= 1:/# => ?.
+  by rewrite (canRL _ _ len{2} i W32.to_uintK) 1:/#.
 qed.
 
 equiv increment_counter: ChaCha20_pref.M.increment_counter ~ ChaCha20_sref.M.increment_counter :
@@ -119,24 +369,26 @@ proof.
 qed.
 
 equiv pref_sref : ChaCha20_pref.M.chacha20_ref ~ ChaCha20_sref.M.chacha20_ref : 
-  ={output, plain, len, key, nonce,counter, Glob.mem} 
+  ={output, plain, len, key, nonce,counter, Glob.mem} /\
+  (inv_ptr output plain len){1}
   ==>
   ={Glob.mem}.
 proof.
 proc => /=.
-sp; seq 1 1 : (#pre /\ ={st}).
-+ call init;skip => />.
+sp; seq 1 1 : (#{/~(_ = witness)}pre /\ ={st}).
++ by call init;skip => />.
 splitwhile{1} 1 : (W32.of_int 64 \ule len).
 seq 1 1 : (={st, Glob.mem} /\ 
            output{1} = s_output{2} /\ plain{1} = s_plain{2} /\ len{1} = s_len{2} /\
            len{1} \ult W32.of_int 64). 
 + while (={st, Glob.mem} /\ 
-          output{1} = s_output{2} /\ plain{1} = s_plain{2} /\ len{1} = s_len{2}).
+          output{1} = s_output{2} /\ plain{1} = s_plain{2} /\ len{1} = s_len{2} /\
+          (inv_ptr output plain len){1}). 
   + call increment_counter;ecall (store len{1}); call sum_states; call rounds; call copy_state.
-    skip => /> &m; rewrite W32.ultE W32.uleE /= => h1 h2 [/=] />.
+    skip => /> &m; rewrite W32.ultE W32.uleE /= => ????????? ->.
     by rewrite W32.uleE W32.ultE /= W32.to_uintB 1:W32.uleE //= /#.
-  skip => /> &m;rewrite W32.uleE W32.ultE /=;split => [/# | s_len_R].
-  rewrite !W32.uleE !W32.ultE /= /#.
+  skip => /> &m;rewrite W32.uleE W32.ultE /= => *;split => [/# | s_len_R out pla].
+  by rewrite !W32.uleE !W32.ultE /= /#.
 unroll{1} 1.
 seq 1 1 : (={Glob.mem} /\ len{1} = W32.of_int 0);last first.
 + by rcondf{1} 1; move=> *;skip => />.
